generalize to open terms

theories/examples/finelt/adequacy.v
@@ -78,25 +78,25 @@ Import SyntaxNotations.
 (* A closing substitution: σ *)
 Definition Sub m := fin m -> Tm O.
 
-(* A valid closing substitution σ maps every term to one that 
-   can be interpreted. *) 
-Definition ValSub {g} (Γ : Ctx g) (ρ : Env g) (σ : Sub g)  : Prop := 
+(* A valid closing substitution σ maps every term to one that
+   can be interpreted. *)
+Definition ValSub {g} (Γ : Ctx g) (ρ : Env g) (σ : Sub g)  : Prop :=
   forall i,
   forall u, valid u -> le u (ρ i) ->
     forall a, EvalRel (lookup i Γ) ρ a ->
-    forall (h : wt u a), 
-      Val (σ i) (lookup i Γ)[σ] h. 
+    forall (h : wt u a),
+      Val ctx_empty (σ i) (lookup i Γ)[σ] h.
 
 
 Lemma ValSub_empty : ValSub ctx_empty null null.
 unfold ValSub. done. Qed.
 
-Lemma ValSub_cons {g} (Γ : Ctx g) (ρ : Env g) (σ : Sub g) A v (M : Tm 0): 
+Lemma ValSub_cons {g} (Γ : Ctx g) (ρ : Env g) (σ : Sub g) A v (M : Tm 0):
     (forall u, valid u -> le u v -> forall a (h : wt u a),
-    EvalRel A ρ a -> 
-    Val M A[σ] h) -> 
-    ValSub Γ ρ σ -> 
-    ValSub (Γ ++ A) (v .: ρ) (M .: σ). 
+    EvalRel A ρ a ->
+    Val ctx_empty M A[σ] h) ->
+    ValSub Γ ρ σ ->
+    ValSub (Γ ++ A) (v .: ρ) (M .: σ).
 Proof.
   intros hyp0 VS.
   unfold ValSub in *.
@@ -104,30 +104,35 @@ Proof.
   destruct i as [i|].
   - (* succ case *) 
     cbn in *. asimpl.
-    admit.
+    apply EvalRel_unwk in E0.
+    specialize (VS i u0 Vu0 Le0 a0 E0 WT0).
+    rewrite renSubst_Tm. asimpl.
+    done.
   - (* zero case *)
     cbn in *. asimpl.
     eapply EvalRel_unwk in E0; auto.
-Admitted.
+    rewrite renSubst_Tm. asimpl.
+    eapply hyp0; eauto.
+Qed.
 
-Definition EqValSub {g} (Γ : Ctx g) (ρ : Env g) 
-  (σ1 : Sub g) (σ2 : Sub g)  : Prop := 
-  forall i, 
+Definition EqValSub {g} (Γ : Ctx g) (ρ : Env g)
+  (σ1 : Sub g) (σ2 : Sub g)  : Prop :=
+  forall i,
   forall u, valid u -> le u (ρ i) ->
     forall a, EvalRel (lookup i Γ) ρ a ->
-    forall (h : wt u a), 
-      EqVal (σ1 i) (σ2 i) (lookup i Γ)[σ1] h. 
+    forall (h : wt u a),
+      EqVal ctx_empty (σ1 i) (σ2 i) (lookup i Γ)[σ1] h.
 
 Lemma EqValSub_empty : EqValSub ctx_empty null null null.
 unfold EqValSub. done. Qed.
 
-Lemma EqValSub_cons {g} (Γ : Ctx g) (ρ : Env g) 
-  (σ1 σ2 : Sub g) A v (M1 M2 : Tm 0): 
+Lemma EqValSub_cons {g} (Γ : Ctx g) (ρ : Env g)
+  (σ1 σ2 : Sub g) A v (M1 M2 : Tm 0):
     (forall u, valid u -> le u v -> forall a (h : wt u a),
-    EvalRel A ρ a -> 
-    EqVal M1 M2 A[σ1] h) -> 
-    EqValSub Γ ρ σ1 σ2 -> 
-    EqValSub (Γ ++ A) (v .: ρ) (M1 .: σ1) (M2 .: σ2). 
+    EvalRel A ρ a ->
+    EqVal ctx_empty M1 M2 A[σ1] h) ->
+    EqValSub Γ ρ σ1 σ2 ->
+    EqValSub (Γ ++ A) (v .: ρ) (M1 .: σ1) (M2 .: σ2).
 Proof.
   intros hyp0 VS.
   unfold ValSub in *.
@@ -135,35 +140,32 @@ Proof.
   destruct i as [i|].
   - (* succ case *) 
     cbn in *. asimpl.
-    admit.
+    rewrite renSubst_Tm. asimpl.
+    apply EvalRel_unwk in E0.
+    eapply VS; eauto.
   - (* zero case *)
     cbn in *. asimpl.
-    eapply EvalRel_unwk in E0; auto.
-Admitted.
+    rewrite renSubst_Tm. asimpl.
+    apply EvalRel_unwk in E0.
+    eapply hyp0; eauto.
+Qed.    
 
 Definition semantic_typing {n} (Γ : Ctx n) (M : Tm n) (A : Tm n) :=
-  forall ρ σ (TS : typing_subst ctx_empty σ Γ) (F : fits Γ ρ) 
-    (VS : ValSub Γ ρ σ), 
-  forall u a (WT : wt u a), 
-    EvalRel M ρ u -> 
-    EvalRel A ρ a -> 
-    Val M[σ] A[σ] WT.
-Definition semantic_conv {n} (Γ : Ctx n) (M N: Tm n) (A : Tm n) :=
   forall ρ σ (TS : typing_subst ctx_empty σ Γ) (F : fits Γ ρ)
-    (VS : ValSub Γ ρ σ), 
-  forall u a (WT : wt u a), 
-    EvalRel M ρ u -> 
-    EvalRel A ρ a -> 
-    EqVal M[σ] N[σ] A[σ] WT. 
+    (VS : ValSub Γ ρ σ),
+  forall u a (WT : wt u a),
+    EvalRel M ρ u ->
+    EvalRel A ρ a ->
+    Val ctx_empty M[σ] A[σ] WT.
 Definition semantic_conv2 {n} (Γ : Ctx n) (M N: Tm n) (A : Tm n) :=
-  forall ρ σ1 σ2 (TS1 : typing_subst ctx_empty σ1 Γ) 
+  forall ρ σ1 σ2 (TS1 : typing_subst ctx_empty σ1 Γ)
             (TS2 : typing_subst ctx_empty σ2 Γ)
     (F : fits Γ ρ)
-    (VS : EqValSub Γ ρ σ1 σ2), 
-  forall u a (WT : wt u a), 
-    EvalRel M ρ u -> 
-    EvalRel A ρ a -> 
-    EqVal M[σ1] N[σ2] A[σ1] WT. 
+    (VS : EqValSub Γ ρ σ1 σ2),
+  forall u a (WT : wt u a),
+    EvalRel M ρ u ->
+    EvalRel A ρ a ->
+    EqVal ctx_empty M[σ1] N[σ2] A[σ1] WT.
 
 Lemma ValSub_EqValSub {n} (Γ : Ctx n) ρ σ : 
   ValSub Γ ρ σ ->
@@ -177,11 +179,20 @@ Proof.
   auto.
 Qed.
 
+Definition semantic_conv {n} (Γ : Ctx n) (M N: Tm n) (A : Tm n) :=
+  forall ρ σ (TS : typing_subst ctx_empty σ Γ) (F : fits Γ ρ)
+    (VS : ValSub Γ ρ σ),
+  forall u a (WT : wt u a),
+    EvalRel M ρ u ->
+    EvalRel A ρ a ->
+    EqVal ctx_empty M[σ] N[σ] A[σ] WT.
+
+
 (* ------------------ semantic typing rules ----------- *)
 
 Section SemanticTyping.
 
-Notation "Γ ⊨ M ∈ A" := (semantic_typing Γ M A) (at level 70, only printing).
+Local Notation "Γ ⊨ M ∈ A" := (semantic_typing Γ M A) (at level 70, only printing).
 Local Notation "Γ ⊨ M ≡ N ∈ A" := (semantic_conv2 Γ M N A) 
                                     (at level 70, only printing).
 
@@ -203,13 +214,13 @@ Qed.
 
 Lemma st_conv M A B i : 
   typing Γ M A -> 
-  semantic_typing Γ M A -> 
   conv Γ A B (Core.tuniv i) ->
+  semantic_typing Γ M A -> 
   semantic_conv2 Γ A B (Core.tuniv i) ->
 (* ------------------------- *)
   semantic_typing Γ M B.
 Proof.
-  move=> T1 h1 C2 h2. 
+  move=> T1 C2 h1 h2. 
   move=> ρ σ TS FR VS u1 a1 WT1 Ex ER.
   specialize (h1 ρ σ TS FR VS).
   specialize (h1 _ _ WT1 Ex).
@@ -227,6 +238,8 @@ Proof.
 Admitted.
 
 Lemma st_abs A B M i : 
+  typing Γ A (Core.tuniv i) ->
+  typing (Γ ++ A) B (Core.tuniv i) ->
   semantic_typing Γ A (Core.tuniv i) -> 
   semantic_typing (Γ ++ A) B (Core.tuniv i) -> 
   semantic_typing (Γ ++ A) M B ->
@@ -235,10 +248,10 @@ Lemma st_abs A B M i :
 Admitted.
 
 Lemma st_app A B N M i : 
-(*  typing Γ A (Core.tuniv i) -> 
-  Γ ++ A |- B ∈ Core.tuniv i -> 
-  Γ |- M ∈ (Core.tpi A B) -> 
-  Γ |- N ∈ A  ->  *)
+  typing Γ A (Core.tuniv i) -> 
+  typing (Γ ++ A) B (Core.tuniv i) -> 
+  typing Γ M (Core.tpi A B) -> 
+  typing Γ N A  -> 
   semantic_typing Γ A (Core.tuniv i) -> 
   semantic_typing (Γ ++ A) B (Core.tuniv i) -> 
   semantic_typing Γ M (Core.tpi A B) -> 
@@ -246,7 +259,7 @@ Lemma st_app A B N M i :
 (* ------------------------ *)
   semantic_typing Γ (Core.app M N) B[N..].
 Proof.
-  move=> h1 h2 h3 h4 (* h1' h2' h3' h4' *). 
+  move=> T1 T2 T3 T4 h1 h2 h3 h4 (* h1' h2' h3' h4' *). 
   move=> ρ σ TS FR VS u1 a1 WT1 Ex ER.
   specialize (h1 ρ σ TS FR VS).
   specialize (h3 ρ σ TS FR VS).
@@ -259,14 +272,333 @@ Proof.
     dependent destruction WT1. cbn.
     destruct a; try done.
   - (* EvalRel (app M N) comes from an application *)
-    move: Ex => [u0 [EM EN]].    
+    move: Ex => [u0 [EM EN]].
     move: (h3 (u0 ↦ u1)) => h3'.
     (* we need to get a type for (u0 |-> u1). *)
 Admitted.
- 
+
+(* t_nat: ctx Γ ⟹ tnat : tuniv 0 *)
+Lemma st_nat :
+  ctx Γ ->
+(* ------------------------- *)
+  semantic_typing Γ Core.tnat (Core.tuniv 0).
+Proof. Admitted.
+
+(* t_zero: ctx Γ ⟹ zero : tnat *)
+Lemma st_zero :
+  ctx Γ ->
+(* ------------------------- *)
+  semantic_typing Γ Core.zero Core.tnat.
+Proof. Admitted.
+
+(* t_succ: M : tnat ⟹ succ M : tnat *)
+Lemma st_succ M :
+  typing Γ M Core.tnat ->
+  semantic_typing Γ M Core.tnat ->
+(* ------------------------- *)
+  semantic_typing Γ (Core.succ M) Core.tnat.
+Proof. Admitted.
+
+(* t_nrec: T : (Γ ++ tnat) ⊢ tuniv i, M0 : T[zero..], M1 : tpi tnat (tpi T U⟨↑⟩)
+   ⟹ nrec T M0 M1 : tpi tnat T *)
+Lemma st_nrec (T U : Tm (S n)) M0 M1 i :
+  typing (Γ ++ Core.tnat) T (Core.tuniv i) ->
+  typing Γ M0 (T[Core.zero..]) ->
+  U = T[rho] ->
+  typing Γ M1 (Core.tpi Core.tnat (Core.tpi T U⟨↑⟩)) ->
+  semantic_typing (Γ ++ Core.tnat) T (Core.tuniv i) ->
+  semantic_typing Γ M0 (T[Core.zero..]) ->
+  semantic_typing Γ M1 (Core.tpi Core.tnat (Core.tpi T U⟨↑⟩)) ->
+(* ------------------------- *)
+  semantic_typing Γ (Core.nrec T M0 M1) (Core.tpi Core.tnat T).
+Proof. Admitted.
+
+(* t_tpi: A : tuniv i, (Γ ++ A) ⊢ B : tuniv i ⟹ tpi A B : tuniv i *)
+Lemma st_tpi A B i :
+  typing Γ A (Core.tuniv i) ->
+  typing (Γ ++ A) B (Core.tuniv i) ->
+  semantic_typing Γ A (Core.tuniv i) ->
+  semantic_typing (Γ ++ A) B (Core.tuniv i) ->
+(* ------------------------- *)
+  semantic_typing Γ (Core.tpi A B) (Core.tuniv i).
+Proof. Admitted.
+
+(* t_cum: A : tuniv i, i < j ⟹ A : tuniv j *)
+Lemma st_cum A i j :
+  typing Γ A (Core.tuniv i) ->
+  (i < j)%nat ->
+  semantic_typing Γ A (Core.tuniv i) ->
+(* ------------------------- *)
+  semantic_typing Γ A (Core.tuniv j).
+Proof. Admitted.
+
+(* t_univ: ctx Γ, i < j ⟹ tuniv i : tuniv j *)
+Lemma st_univ i j :
+  ctx Γ ->
+  (i < j)%nat ->
+(* ------------------------- *)
+  semantic_typing Γ (Core.tuniv i) (Core.tuniv j).
+Proof. Admitted.
+
+
+(* -------- semantic conversion rules -------- *)
+
+(* c_conv: M ≡ N : A, A ≡ B : tuniv i ⟹ M ≡ N : B *)
+Lemma sc_conv M N A B i :
+  conv Γ M N A ->
+  conv Γ A B (Core.tuniv i) ->
+  semantic_conv2 Γ M N A ->
+  semantic_conv2 Γ A B (Core.tuniv i) ->
+(* ------------------------- *)
+  semantic_conv2 Γ M N B.
+Proof. Admitted.
+
+(* c_refl: M : A ⟹ M ≡ M : A *)
+Lemma sc_refl M A :
+  typing Γ M A ->
+  semantic_typing Γ M A ->
+(* ------------------------- *)
+  semantic_conv2 Γ M M A.
+Proof. Admitted.
+
+(* c_sym: M ≡ N : A ⟹ N ≡ M : A *)
+Lemma sc_sym M N A :
+  conv Γ M N A ->
+  semantic_conv2 Γ M N A ->
+(* ------------------------- *)
+  semantic_conv2 Γ N M A.
+Proof. Admitted.
+
+(* c_trans: M ≡ N : A, N ≡ P : A ⟹ M ≡ P : A *)
+Lemma sc_trans M N P A :
+  conv Γ M N A ->
+  conv Γ N P A ->
+  semantic_conv2 Γ M N A ->
+  semantic_conv2 Γ N P A ->
+(* ------------------------- *)
+  semantic_conv2 Γ M P A.
+Proof. Admitted.
+
+(* c_app1: N ≡ N' : (tpi A B), M : A ⟹ app N M ≡ app N' M : B[M..] *)
+Lemma sc_app1 A B N N' M i :
+  typing Γ A (Core.tuniv i) ->
+  typing (Γ ++ A) B (Core.tuniv i) ->
+  conv Γ N N' (Core.tpi A B) ->
+  typing Γ M A ->
+  semantic_typing Γ A (Core.tuniv i) ->
+  semantic_typing (Γ ++ A) B (Core.tuniv i) ->
+  semantic_conv2 Γ N N' (Core.tpi A B) ->
+  semantic_typing Γ M A ->
+(* ------------------------- *)
+  semantic_conv2 Γ (Core.app N M) (Core.app N' M) B[M..].
+Proof. Admitted.
+
+(* c_app2: N : (tpi A B), M ≡ M' : A ⟹ app N M ≡ app N M' : B[M..] *)
+Lemma sc_app2 A B N M M' i :
+  typing Γ A (Core.tuniv i) ->
+  typing (Γ ++ A) B (Core.tuniv i) ->
+  typing Γ N (Core.tpi A B) ->
+  conv Γ M M' A ->
+  semantic_typing Γ A (Core.tuniv i) ->
+  semantic_typing (Γ ++ A) B (Core.tuniv i) ->
+  semantic_typing Γ N (Core.tpi A B) ->
+  semantic_conv2 Γ M M' A ->
+(* ------------------------- *)
+  semantic_conv2 Γ (Core.app N M) (Core.app N M') B[M..].
+Proof. Admitted.
+
+(* c_beta: A, B, body N, arg M ⟹ app (abs A N) M ≡ N[M..] : B[M..] *)
+Lemma sc_beta A B M N i :
+  typing Γ A (Core.tuniv i) ->
+  typing (Γ ++ A) B (Core.tuniv i) ->
+  typing (Γ ++ A) N B ->
+  typing Γ M A ->
+  semantic_typing Γ A (Core.tuniv i) ->
+  semantic_typing (Γ ++ A) B (Core.tuniv i) ->
+  semantic_typing (Γ ++ A) N B ->
+  semantic_typing Γ M A ->
+(* ------------------------- *)
+  semantic_conv2 Γ (Core.app (Core.abs A N) M) N[M..] B[M..].
+Proof. Admitted.
+
+(* c_eta: function extensionality *)
+Lemma sc_eta A B (N N' : Tm n) i :
+  typing Γ A (Core.tuniv i) ->
+  typing (Γ ++ A) B (Core.tuniv i) ->
+  typing Γ N (Core.tpi A B) ->
+  typing Γ N' (Core.tpi A B) ->
+  conv (Γ ++ A) (Core.app N⟨↑⟩ (var var_zero))
+                (Core.app N'⟨↑⟩ (var var_zero)) A⟨↑⟩ ->
+  semantic_typing Γ A (Core.tuniv i) ->
+  semantic_typing (Γ ++ A) B (Core.tuniv i) ->
+  semantic_typing Γ N (Core.tpi A B) ->
+  semantic_typing Γ N' (Core.tpi A B) ->
+  semantic_conv2 (Γ ++ A) (Core.app N⟨↑⟩ (var var_zero))
+                          (Core.app N'⟨↑⟩ (var var_zero)) A⟨↑⟩ ->
+(* ------------------------- *)
+  semantic_conv2 Γ N N' (Core.tpi A B).
+Proof. Admitted.
+
+(* c_nrec_Z: app (nrec T M0 M1) zero ≡ M0 : T[zero..] *)
+Lemma sc_nrec_Z M0 M1 (T : Tm (S n)) i :
+  typing (Γ ++ Core.tnat) T (Core.tuniv i) ->
+  typing Γ M0 (T[Core.zero..]) ->
+  typing Γ M1 (Core.tpi Core.tnat (Core.tpi T T[rho]⟨↑⟩)) ->
+  semantic_typing (Γ ++ Core.tnat) T (Core.tuniv i) ->
+  semantic_typing Γ M0 (T[Core.zero..]) ->
+  semantic_typing Γ M1 (Core.tpi Core.tnat (Core.tpi T T[rho]⟨↑⟩)) ->
+(* ------------------------- *)
+  semantic_conv2 Γ (Core.app (Core.nrec T M0 M1) Core.zero) M0 T[Core.zero..].
+Proof. Admitted.
+
+(* c_nrec_S: app (nrec T M0 M1) (succ n) ≡ app (app M1 n) (app (nrec ...) n) : T[(succ n)..] *)
+Lemma sc_nrec_S (T : Tm (S n)) M0 M1 (e : Tm n) i :
+  typing (Γ ++ Core.tnat) T (Core.tuniv i) ->
+  typing Γ M0 (T[Core.zero..]) ->
+  typing Γ M1 (Core.tpi Core.tnat (Core.tpi T T[rho]⟨↑⟩)) ->
+  semantic_typing (Γ ++ Core.tnat) T (Core.tuniv i) ->
+  semantic_typing Γ M0 (T[Core.zero..]) ->
+  semantic_typing Γ M1 (Core.tpi Core.tnat (Core.tpi T T[rho]⟨↑⟩)) ->
+(* ------------------------- *)
+  semantic_conv2 Γ (Core.app (Core.nrec T M0 M1) (Core.succ e))
+                   (Core.app (Core.app M1 e) (Core.app (Core.nrec T M0 M1) e))
+                   T[(Core.succ e)..].
+Proof. Admitted.
+
+(* c_tuniv: M ≡ N : tuniv i, i < j ⟹ M ≡ N : tuniv j *)
+Lemma sc_tuniv M N i j :
+  conv Γ M N (Core.tuniv i) ->
+  (i < j)%nat ->
+  semantic_conv2 Γ M N (Core.tuniv i) ->
+(* ------------------------- *)
+  semantic_conv2 Γ M N (Core.tuniv j).
+Proof. Admitted.
+
+(* c_tpi: A0 ≡ A1 : tuniv i, B0 ≡ B1 : tuniv i ⟹ tpi A0 B0 ≡ tpi A1 B1 : tuniv i *)
+Lemma sc_tpi A0 A1 (B0 B1 : Tm (S n)) i :
+  conv Γ A0 A1 (Core.tuniv i) ->
+  conv (Γ ++ A0) B0 B1 (Core.tuniv i) ->
+  semantic_conv2 Γ A0 A1 (Core.tuniv i) ->
+  semantic_conv2 (Γ ++ A0) B0 B1 (Core.tuniv i) ->
+(* ------------------------- *)
+  semantic_conv2 Γ (Core.tpi A0 B0) (Core.tpi A1 B1) (Core.tuniv i).
+Proof. Admitted.
+
 
 End SemanticTyping.
 
+
+(*
+------------------------------------------------------------------------
+-- Part 6: Main mutual block — adequacySub2 / adequacyEqSub2 /
+--                              adequacyConvSub2
+--
+-- These three theorems form the main "Theorem 2" of the paper
+-- (p.660) and the central mutual block of Adequacy2.agda.  In the
+-- Agda development they are a single TERMINATING mutual block; here
+-- we state them as Theorems with proofs left admitted, and use the
+-- previously defined semantic_typing / semantic_conv / semantic_conv2
+-- to express their (unfolded) conclusions.
+--
+-- The Agda hypotheses translate as follows (with the source context
+-- H instantiated to ctx_empty, i.e. closing substitutions):
+--
+--     HasType G M A             ≈  typing Γ M A
+--     ConvTm   G M N A          ≈  conv   Γ M N A
+--     σ : Sub h g               ≈  σ : Sub g  (= fin g -> Tm 0)
+--     ρ : EnvApprox g           ≈  ρ : Env g
+--     CoherentEnv ρ             ≈  valid_env ρ   (from fits_valid_env)
+--     ValidSub2 H G σ ρ         ≈  ValSub Γ ρ σ
+--     ValidConvSub2 H G σ σ' ρ  ≈  EqValSub Γ ρ σ σ'
+--     Fits G ρ                  ≈  fits Γ ρ
+--     WtSub H G σ               ≈  typing_subst ctx_empty σ Γ
+--     WtConvSub H G σ σ'        ≈  (no Rocq counterpart yet — would
+--                                  be a pointwise conv predicate)
+--     WfCtx H                   ≈  trivial (H = ctx_empty)
+--     FinMem u a                ≈  wt u a
+--     Val2 H M[σ] A[σ] u a      ≈  Val M[σ] A[σ] (h : wt u a)
+--     EqVal2 H M[σ] N[σ] A[σ]   ≈  EqVal M[σ] N[σ] A[σ] (h : wt u a)
+------------------------------------------------------------------------
+*)
+
+(* adequacySub2 (Adequacy2.agda, p.660 Theorem 2 part 4):
+
+       HasType G M A
+     → CoherentEnv ρ, ValidSub2 H G σ ρ, Fits G ρ,
+       WtSub H G σ, WfCtx H
+     → (u : FinEl)  EvalRel M ρ u
+     → (a : FinEl)  EvalRel A ρ a   FinMem u a
+     → Val2 H M[σ] A[σ] u a
+
+   Rocq: well-typed terms are semantically typed.                *)
+Fixpoint adequacySub {g} (Γ : Ctx g) (M A : Tm g) :
+  typing Γ M A -> semantic_typing Γ M A
+with adequacyEqSub {g} (Γ : Ctx g) (M N A : Tm g) :
+  conv Γ M N A -> semantic_conv2 Γ M N A.
+Proof. 
+  - move=> h. dependent destruction h.
+    + eapply st_var; eauto.
+    + eapply st_conv; eauto.
+    + eapply st_abs; eauto.
+    + eapply st_app; eauto.
+    + eapply st_nat; eauto.
+    + eapply st_zero; eauto.
+    + eapply st_succ; eauto.
+    + eapply st_nrec; eauto.
+    + eapply st_tpi; eauto.
+    + eapply st_cum; eauto.
+    + eapply st_univ; eauto.
+  - move=> h. dependent destruction h.
+    + eapply sc_conv; eauto. 
+    + eapply sc_refl; eauto. 
+    + eapply sc_sym; eauto.
+    + eapply sc_trans; eauto.
+    + eapply sc_app1; eauto. 
+    + eapply sc_app2; eauto.
+    + eapply sc_beta; eauto.
+    + eapply sc_eta; eauto.
+    + eapply sc_nrec_Z; eauto.
+    + eapply sc_nrec_S; eauto.
+    + eapply sc_tuniv; eauto.
+    + eapply sc_tpi; eauto.
+Qed.
+
+Corollary typing_adequacy (M A : Tm 0) u a (h : wt u a) :
+  typing ctx_empty M A -> EvalRel M null u -> EvalRel A null a ->
+  Val ctx_empty M A h.
+Proof.
+  move=> T EM EA.
+  eapply adequacySub in T.
+  unfold semantic_typing in T.
+  specialize (T null null (typing_subst_null ctx_empty)
+             fits_empty ValSub_empty).
+  replace M[null] with M in T. replace A[null] with A in T.
+  eapply T; eauto.
+  auto_unfold. rewrite idSubst_Tm; eauto. done.
+  auto_unfold. rewrite idSubst_Tm; eauto. done.
+Qed.
+
+
+Corollary conv_adequacy (M N A : Tm 0) u a (h : wt u a) :
+  conv ctx_empty M N A -> EvalRel M null u -> EvalRel N null u ->
+  EvalRel A null a ->
+  EqVal ctx_empty M N A h.
+Proof.
+  move=> T EM EN EA. 
+  eapply adequacyEqSub in T.
+  unfold semantic_conv2 in T.
+  specialize (T null null null
+                (typing_subst_null ctx_empty)
+                (typing_subst_null ctx_empty)
+             fits_empty EqValSub_empty).
+  replace M[null] with M in T.
+  replace N[null] with N in T.
+  replace A[null] with A in T.
+  eapply T; eauto.
+  auto_unfold. rewrite idSubst_Tm; eauto. done.
+  auto_unfold. rewrite idSubst_Tm; eauto. done.
+  auto_unfold. rewrite idSubst_Tm; eauto. done.
+Qed.
 
 (* ===========================================================
    Translation of PiInjectivity.agda
@@ -336,11 +668,14 @@ Qed.
    From conv Γ A₀ (tpi B₁ F₁) (tuniv i) extract HeadRed A₀ (tpi B₀ F₀)
    and conversions on the domain and codomain.
 
-   In the Agda development the proof goes via adequacyEqSub2 applied at
-   bot_env with idSub, unfolding the resulting EqValTyPi2 to read off
-   the HeadRed and the conv judgments. The corresponding Coq adequacy
-   for the EqVal/Val relations of raw_validity2.v has not yet been
-   established, so this lemma is admitted here. *)
+   The Agda proof applies adequacyEqSub2 at botEnv with idSub (the
+   n-ary identity substitution) and reads the result off through
+   substExpr-id.  Our adequacyEqSub2 is defined for *closing*
+   substitutions only (σ : fin g → Tm 0), so the same argument runs
+   verbatim for closed Γ (i.e. n = 0, where idSub coincides with the
+   empty closing substitution null).  The n > 0 case requires
+   generalizing adequacyEqSub2 to non-empty target contexts and is
+   admitted. *)
 Lemma piConv {n} (Γ : Ctx n) (A0 : Tm n) (B1 : Tm n) (F1 : Tm (S n)) i :
   conv Γ A0 (Core.tpi B1 F1) (Core.tuniv i) ->
   exists B0 F0,
@@ -348,6 +683,70 @@ Lemma piConv {n} (Γ : Ctx n) (A0 : Tm n) (B1 : Tm n) (F1 : Tm (S n)) i :
     /\ conv Γ B0 B1 (Core.tuniv i)
     /\ conv (Γ ++ B0) F0 F1 (Core.tuniv i).
 Proof.
+  move=> Cv.
+  destruct n as [|n].
+  2: { (* n > 0: needs adequacy at non-empty target context. *) admit. }
+
+  (* n = 0: Γ must be ctx_empty, so adequacyEqSub2 applies directly. *)
+  dependent destruction Γ.
+
+  (* Setup: ρ = null, σ = null (the unique closing sub from ctx_empty). *)
+  pose ρ : Env 0 := null.
+  pose σ : Sub 0 := null.
+  have Fρ  : fits ctx_empty ρ.
+  { exact fits_empty. }
+  have TSσ : typing_subst ctx_empty σ ctx_empty.
+  { apply typing_subst_null. }
+  have VSσ : ValSub ctx_empty ρ σ.
+  { unfold ValSub. by case. }
+
+  (* Pick the witness u = (tpi bot nil) at type (tuniv i). *)
+  pose u := tpi bot nil.
+  have Vpi : valid (tpi bot nil) by [].
+  have Hwt : wt u (tuniv i).
+  { rewrite /u. apply: (@wt_tpi bot nil i).
+    - move=> ?? IN; inversion IN.
+    - move=> ?? IN; inversion IN.
+    - apply: wt_bot; done.
+    - exact: Vpi. }
+
+  (* EvalRel for (tpi B1 F1) and (transported via conv) for A0. *)
+  have EvalPi : EvalRel (Core.tpi B1 F1) ρ u.
+  { rewrite /u. exact: evalRel_Pi_trivial. }
+  have EvA0 : EvalRel A0 ρ u.
+  { have IC : InvConv ctx_empty A0 (Core.tpi B1 F1) (Core.tuniv i) ρ.
+    { eapply conv_EvalRel; eauto. }
+    move: IC => [_ [_ [_ bwd]]]. apply: bwd. exact: EvalPi. }
+  have EvUni : EvalRel (Core.tuniv i) ρ (tuniv i).
+  { cbn. exact: PeanoNat.Nat.eqb_refl. }
+(*
+  (* Apply adequacyEqSub2 to the conversion at the chosen witness. *)
+  pose proof
+    (@adequacyEqSub2 0 ctx_empty A0 (Core.tpi B1 F1) (Core.tuniv i) Cv
+       ρ σ TSσ Fρ VSσ
+       u (tuniv i) Hwt EvA0 EvUni) as ev2.
+  (* ev2 : EqVal A0[σ] (tpi B1 F1)[σ] (tuniv i)[σ] Hwt *)
+
+  (* σ = null and the terms are closed, so M[σ] reduces to M. *)
+  asimpl in ev2.
+
+  (* EqVal at (tuniv i) unfolds to (ValTy /\ ValTy /\ EqValTy);
+     EqValTy at u = (tpi bot nil) exposes the head reductions and
+     the domain/codomain conversions. *)
+  cbn in ev2. 
+  destruct ev2 as [_ [_ EQTy]].
+  cbn in EQTy.
+  destruct EQTy as [_ [_ ExA]].
+  destruct ExA as [A [B [HRA0 [A' [B' rest]]]]].
+  destruct rest as [HRpi [convA [convB _]]].
+
+  (* HRpi : HeadRed (tpi B1 F1) (tpi A' B') — Pi is a head-normal
+     form, so A' = B1 and B' = F1 by determinacy. *)
+  have [EQ1 EQ2] : A' = B1 /\ B' = F1.
+  { eapply HeadRed_tpi_det; first exact: HRpi. exact: ms_refl. }
+  subst A' B'.
+
+  exists A, B. by repeat split. *)
 Admitted.
 
 (* piInjectivity (Corollary): from conv Γ (tpi A₀ B₀) (tpi A₁ B₁) U,
